Test/dafny0/ComputationsNeg.dfy
@@ -2,13 +2,13 @@
 // RUN: %diff "%s.expect" "%t"
 
 function bad(n: nat): nat
-  decreases n;
+  decreases n
 {
-  bad(n+1)
+  bad(n+1)  // error: termination failure
 }
 ghost method go_bad()
-  ensures bad(0)==0;
-{
+  ensures bad(0)==0
+{  // error: postcondition violation
 }
 
 datatype Nat = Zero | Succ(tail: Nat)
@@ -16,17 +16,17 @@ predicate ThProperty(step: nat, t: Nat, r: nat)
 {
   match t
   case Zero => true
-  case Succ(o) => step>0 && exists ro:nat, ss :: ss == step-1 ==> ThProperty(ss, o, ro) // WISH: auto-generate ss
+  case Succ(o) => step>0 && exists ro:nat, ss :: ss == step-1 && ThProperty(ss, o, ro) // WISH: auto-generate ss
 }
 ghost method test_ThProperty()
-  ensures ThProperty(10, Succ(Zero), 0);
-{
+  ensures ThProperty(10, Succ(Zero), 0)
+{  // error: postcondition violation
 //  assert ThProperty(9, Zero, 0);
 }
 
 // The following is a test that well-typedness antecednets are included in the literal axioms
 function StaticFact(n: nat): nat
-  ensures 0 < StaticFact(n);
+  ensures 0 < StaticFact(n)
 {
   if n == 0 then 1 else n * StaticFact(n - 1)
 }
